Implementation of warps

Execution_resources.v
@@ -1,38 +1,24 @@
 
 From Views Require Import utils.
 Require Import PeanoNat.
-From Views Require Import BoundedInt.
 
 
-
-
-(* Inductive execlevel: Type :=
-  | Blocks
-  | Warps
-  | Threads.
-Inductive filtersize: Type := FilterSize (l: execlevel) (d size: nat).
-Inductive execty: Type :=
-  | TyGpuGrid {num_dims : nat} (gs bs : @DimSizes num_dims) (filtersizes: list filtersize)
-  | TyHostThread.
-Inductive execrange: Type := Range (lower upper: nat) (is_distrib: bool).
-Inductive filter: Type := Filter (l: execlevel) (d: nat) (r: execrange).
-Inductive execexpr: Type :=
-  | HostThread
-  | GpuGrid {num_dims : nat} (grid_size block_size : @DimSizes num_dims) (filter: list filter)
-  | ExecVar (ident: string).
-Inductive exec_distrib: Type :=
-  | Distrib (ed: exec_distrib) (distribs: list (execlevel * nat)). *)
-
-
+Definition Warp_size : nat.
+apply 0.
+Qed.
 
 Definition shape : Type := nat * nat * nat.
-Notation "XYZ< x y z >" := (x,y,z).
+(* Notation "XYZ< x y z >" := (x,y,z).
 Notation "XY< x y >" := (x,y,1).
 Notation "XZ< x z >" := (x,1,z).
 Notation "YZ< y z >" := (1,y,z).
 Notation "X< x >" := (x,1,1).
 Notation "Y< y >" := (1,y,1).
-Notation "Z< z >" := (1,1,z).
+Notation "Z< z >" := (1,1,z). *)
+
+Definition size (shp : shape) :=
+  match shp with | (x,y,z) => x*y*z
+end.
 
 Definition XYZ (x y z : nat) := (x,y,z).
 Definition XY (x y : nat) := (x,y,1).
@@ -42,7 +28,7 @@ Definition X (x : nat) := (x,1,1).
 Definition Y (y : nat) := (1,y,1).
 Definition Z (z : nat) := (1,1,z).
 
-Definition Matrix (T : Type) (shp : shape) : Type :=
+Definition Tensor (T : Type) (shp : shape) : Type :=
   match shp with | (x,y,z) => nat -> nat -> nat -> T
 end.
 
@@ -50,68 +36,87 @@ Definition Vector (T : Type) (n : nat) : Type :=
   nat -> T
 .
 
-Definition Thread_t : Type := nat.
-Definition Warp_t (n : nat) : Type := Vector Thread_t n.
+Definition PhysicalId_t : Type := nat.
+Definition LogicalId_t : Type := nat*nat*nat.
+Definition ThreadId_t : Type := LogicalId_t*LogicalId_t.
+
+Definition Thread_t : Type := LogicalId_t * LogicalId_t.
+Definition PhysThread_t : Type := PhysicalId_t.
+Definition Warp_t : Type := Vector PhysThread_t Warp_size.
 Definition Block_t (shp : shape) : Type :=
-      match shp with | (x,y,z) => Matrix Thread_t (x, y, z) end.
+      match shp with | (x,y,z) => Tensor Thread_t (x, y, z) end.
 Definition Grid_t (shp : shape) (shp' : shape) : Type :=
-      match shp with | (x,y,z) => Matrix (Block_t shp') (x, y, z) end.
+      match shp with | (x,y,z) => Tensor (Block_t shp') (x, y, z) end.
 
 Inductive execution_resource : Type :=
-  | thread (t : Thread_t)
-  | warp (n : nat) (w : Warp_t n)
-  | block (shp : shape) (b : Block_t shp)
+  | thread (t : PhysThread_t)
+  | lthread (t : ThreadId_t)
+  | warp (w : Warp_t)
+  | block (shp : shape) (id : LogicalId_t) (b : Block_t shp)
   | grid (shp : shape) (shp' : shape) (g : Grid_t shp shp')
   | Collection (n : nat) (content : Vector execution_resource n)
   | Error
 .
 
 
-Definition build_block (shp : shape) (offset : nat) : Block_t shp :=
-  match shp with
-  | (x,y,z) => fun i j k => (offset + i + x*j + x*y*k)
+Definition build_block (shp : shape) (id : LogicalId_t) : Block_t shp :=
+  match shp,id with
+  | (x,y,z),(id_x,id_y,id_z) => fun i j k => ((id_x,id_y,id_z),(i,j,k))
 end.
 
 Definition build_grid (shp : shape) (shp' : shape) : Grid_t shp shp' :=
   match shp with
-  | (x,y,z) => fun i j k => (build_block shp' (i + x* j + x*y*k))
+  | (x,y,z) => fun i j k => (build_block shp' (i,j,k))
 end.
 
-Definition build_warp (n : nat) : Warp_t n :=
-  fun i => i
+Definition build_warp (id : nat) : Warp_t :=
+  fun i => (Warp_size*id) + i
 .
 
-Definition Thread (id : nat) := thread id.
-Definition Warp (sz : nat) := warp sz (build_warp sz).
-Definition Block (shp : shape) := block shp (build_block shp 0).
+Definition Thread (id : PhysicalId_t) := thread id.
+Definition LThread (id : ThreadId_t) := lthread id.
+Definition Warp (id : PhysicalId_t) := warp (build_warp id).
+Definition Block (shp : shape) := block shp (0,0,0) (build_block shp (0,0,0)).
+Definition Block' (shp : shape) (id : LogicalId_t) := block shp id (build_block shp id).
 Definition Grid (shp : shape) (shp' : shape) := grid shp shp' (build_grid shp shp').
 
 Inductive dimension :=
   | _x | _y | _z
 .
 
+Definition address_mapping := LogicalId_t * LogicalId_t -> PhysicalId_t.
+
+Fixpoint build_collection (n : nat) (l : nat) (v : Vector execution_resource l) : execution_resource :=
+  match n with
+  | 0 => Collection l v
+  | S n => match (v n) with
+           | Error => Error
+           | _ => build_collection n l v
+           end
+end.
+
 Fixpoint for_all (e : execution_resource) (d : dimension) : execution_resource :=
   match e,d with
-  | Collection n v,_ => Collection n (fun x => for_all (v x) d)
-  | grid (x,1,1) shp' g, _x => Collection x (fun i => block shp' (g i 0 0))
-  | grid (1,y,1) shp' g, _y => Collection y (fun j => block shp' (g 0 j 0))
-  | grid (1,1,z) shp' g, _z => Collection z (fun k => block shp' (g 0 0 k))
+  | Collection n v,_ => Collection n (fun i => for_all (v i) d)
   | grid (1,_,_) _ _, _x => Error
   | grid (_,1,_) _ _, _y => Error
   | grid (_,_,1) _ _, _z => Error
+  | grid (x,1,1) shp' g, _x => Collection x (fun i => block shp' (i,0,0) (g i 0 0))
+  | grid (1,y,1) shp' g, _y => Collection y (fun j => block shp' (0,j,0) (g 0 j 0))
+  | grid (1,1,z) shp' g, _z => Collection z (fun k => block shp' (0,0,k) (g 0 0 k))
   | grid (x,y,z) shp' g, _x => Collection x (fun i => grid (1,y,z) shp' (fun _ j k => g i j k))
   | grid (x,y,z) shp' g, _y => Collection y (fun j => grid (x,1,z) shp' (fun i _ k => g i j k))
   | grid (x,y,z) shp' g, _z => Collection z (fun k => grid (x,y,1) shp' (fun i j _ => g i j k))
-  | block (x,1,1) b, _x => Collection x (fun i => thread (b i 0 0))
-  | block (1,y,1) b, _y => Collection y (fun j => thread (b 0 j 0))
-  | block (1,1,z) b, _z => Collection z (fun k => thread (b 0 0 k))
-  | block (1,_,_) _, _x => Error
-  | block (_,1,_) _, _y => Error
-  | block (_,_,1) _, _z => Error
-  | block (x,y,z) b, _x => Collection x (fun i => block (1,y,z) (fun _ j k => b i j k))
-  | block (x,y,z) b, _y => Collection y (fun j => block (x,1,z) (fun i _ k => b i j k))
-  | block (x,y,z) b, _z => Collection z (fun k => block (x,y,1) (fun i j _ => b i j k))
-  | warp sz w, _x => Collection sz (fun i => thread (w i))
+  | block (1,_,_) _ _, _x => Error
+  | block (_,1,_) _ _, _y => Error
+  | block (_,_,1) _ _, _z => Error
+  | block (x,1,1) _ b, _x => Collection x (fun i => lthread (b i 0 0))
+  | block (1,y,1) _ b, _y => Collection y (fun j => lthread (b 0 j 0))
+  | block (1,1,z) _ b, _z => Collection z (fun k => lthread (b 0 0 k))
+  | block (x,y,z) (id_x,id_y,id_z) b, _x => Collection x (fun i => block (1,y,z) (id_x+i,id_y,id_z) (fun _ j k => b i j k))
+  | block (x,y,z) (id_x,id_y,id_z) b, _y => Collection y (fun j => block (x,1,z) (id_x,id_y+j,id_z) (fun i _ k => b i j k))
+  | block (x,y,z) (id_x,id_y,id_z) b, _z => Collection z (fun k => block (x,y,1) (id_x,id_y,id_z+k) (fun i j _ => b i j k))
+  | warp w, _x => Collection Warp_size (fun i => thread (w i))
   | _,_ => Error
 end.
 
@@ -141,54 +146,155 @@ Notation "x <=? y" := (leb x y).
 Definition assert (cond : bool) (success : execution_resource) : execution_resource :=
   if cond then success else Error.
 
-Fixpoint select (e : execution_resource) (l : nat) (r : nat) (d : dimension) : execution_resource :=
+Fixpoint select_range (e : execution_resource) (l : nat) (r : nat) (d : dimension) : execution_resource :=
   match e,d with
-  | Collection n v,_ => Collection n (fun x => select (v x) l r d)
-  | grid (x,1,1) shp' g, _x => assert (r <=? x) (Collection (r-l) (fun i => block shp' (g (i+l) 0 0)))
-  | grid (1,y,1) shp' g, _y => assert (r <=? y) (Collection (r-l) (fun j => block shp' (g 0 (j+l) 0)))
-  | grid (1,1,z) shp' g, _z => assert (r <=? z) (Collection (r-l) (fun k => block shp' (g 0 0 (k+l))))
+  | Collection n v,_ => Collection n (fun x => select_range (v x) l r d)
   | grid (1,_,_) _ _, _x => Error
   | grid (_,1,_) _ _, _y => Error
   | grid (_,_,1) _ _, _z => Error
+  | grid (x,1,1) shp' g, _x => assert (r <=? x) (Collection (r-l) (fun i => block shp' (i,0,0) (g (i+l) 0 0)))
+  | grid (1,y,1) shp' g, _y => assert (r <=? y) (Collection (r-l) (fun j => block shp' (0,j,0) (g 0 (j+l) 0)))
+  | grid (1,1,z) shp' g, _z => assert (r <=? z) (Collection (r-l) (fun k => block shp' (0,0,k) (g 0 0 (k+l))))
   | grid (x,y,z) shp' g, _x => assert (r <=? x) (Collection (r-l) (fun i => grid (1,y,z) shp' (fun _ j k => g (i+l) j k)))
   | grid (x,y,z) shp' g, _y => assert (r <=? y) (Collection (r-l) (fun j => grid (x,1,z) shp' (fun i _ k => g i (j+l) k)))
   | grid (x,y,z) shp' g, _z => assert (r <=? z) (Collection (r-l) (fun k => grid (x,y,1) shp' (fun i j _ => g i j (k+l))))
-  | block (x,1,1) b, _x => assert (r <=? x) (Collection (r-l) (fun i => thread (b (i+l) 0 0)))
-  | block (1,y,1) b, _y => assert (r <=? y) (Collection (r-l) (fun j => thread (b 0 (j+l) 0)))
-  | block (1,1,z) b, _z => assert (r <=? z) (Collection (r-l) (fun k => thread (b 0 0 (k+l))))
-  | block (1,_,_) _, _x => Error
-  | block (_,1,_) _, _y => Error
-  | block (_,_,1) _, _z => Error
-  | block (x,y,z) b, _x => assert (r <=? x) (Collection (r-l) (fun i => block (1,y,z) (fun _ j k => b (i+l) j k)))
-  | block (x,y,z) b, _y => assert (r <=? y) (Collection (r-l) (fun j => block (x,1,z) (fun i _ k => b i (j+l) k)))
-  | block (x,y,z) b, _z => assert (r <=? z) (Collection (r-l) (fun k => block (x,y,1) (fun i j _ => b i j (k+l))))
-  | warp sz w, _x => Collection sz (fun i => thread (w i))
+  | block (1,_,_) _ _, _x => Error
+  | block (_,1,_) _ _, _y => Error
+  | block (_,_,1) _ _, _z => Error
+  | block (x,1,1) _ b, _x => assert (r <=? x) (Collection (r-l) (fun i => lthread (b (i+l) 0 0)))
+  | block (1,y,1) _ b, _y => assert (r <=? y) (Collection (r-l) (fun j => lthread (b 0 (j+l) 0)))
+  | block (1,1,z) _ b, _z => assert (r <=? z) (Collection (r-l) (fun k => lthread (b 0 0 (k+l))))
+  | block (x,y,z) (id_x,id_y,id_z) b, _x => assert (r <=? x) (Collection (r-l) (fun i => block (1,y,z) (id_x+i,id_y,id_z) (fun _ j k => b (i+l) j k)))
+  | block (x,y,z) (id_x,id_y,id_z) b, _y => assert (r <=? y) (Collection (r-l) (fun j => block (x,1,z) (id_x,id_y+j,id_z) (fun i _ k => b i (j+l) k)))
+  | block (x,y,z) (id_x,id_y,id_z) b, _z => assert (r <=? z) (Collection (r-l) (fun k => block (x,y,1) (id_x,id_y,id_z+k) (fun i j _ => b i j (k+l))))
+  | warp w, _x => assert (r <=? Warp_size) (Collection (r - l) (fun i => thread (w i)))
   | _,_ => Error
 end.
 
 Example test1 :
   to_list (Block (XZ 2 4)) =
-  @ block (XZ 2 4) (fun i j k : nat => i + 2*j + 2*k).
+  @ block (XZ 2 4) (0,0,0) (fun i j k : nat => ((0,0,0),(i, j, k))).
 Proof.
   simpl.
   reflexivity.
 Qed.
 
-Example test2 :
-  to_list (select (Block (XZ 2 4)) 1 3 _z) =
-  [@ block (X 2) (fun i j _ : nat => i + 2*j + 2) :: @ block (X 2) (fun i j _ : nat => i + 2*j + 4) :: []].
-Proof.
-  simpl.
-  reflexivity.
-Qed.
+Definition get_logical_id (shp : shape) : ThreadId_t -> LogicalId_t :=
+  fun i =>
+  match shp,i with
+  | (x',y',z'),((i,j,k),(i',j',k')) =>
+  (i*x'+i',j*y'+j',k*z'+k')
+end.
 
-Example test3 :
-  to_list (for_all (select (Block (XZ 2 4)) 1 3 _z) _x) =
-  [[@ thread 2 :: @ thread 3 :: []] :: [@ thread 4 :: @ thread 5 :: []] :: []].
+Fixpoint get_physical_id_aux (shp : shape) (x' y' z' : nat) : ThreadId_t -> PhysicalId_t :=
+  fun id =>
+  match shp,x',y',z',id with
+  | (x,y,z),S x',y',z',((i,j,k),(i',j',k')) =>
+    match (S x') mod Warp_size with
+    | 0 => i*(S x')+i' + x*(S x')*(j*y'+j') + x*y*(S x')*y'*(k*z'+k')
+    | S n => get_physical_id_aux (x,y,z) x' y' z' id
+    end
+  | (x,y,z),x',y',z',((i,j,k),(i',j',k')) =>
+    i*x'+i' + x*x'*(j*y'+j') + x*y*x'*y'*(k*z'+k')
+end.
+
+Fixpoint lesser_multiple_aux (n : nat) (m : nat) :=
+  match n with
+  | 0 => 0
+  | S n => match (S n mod m) with
+           | 0 => S n
+           | _ => lesser_multiple_aux n m
+end
+end.
+
+Definition lesser_multiple (n : nat) (m : nat) :=
+  match (n mod m) with
+  | 0 => n
+  | _ => lesser_multiple_aux (n + m) m
+end.
+
+Definition get_physical_id (shp : shape) (shp' : shape) : ThreadId_t -> PhysicalId_t :=
+  fun id =>
+  match shp,shp',id with
+  | (x,y,z),(x',y',z'),((i,j,k),(i',j',k')) =>
+    let w := lesser_multiple x' Warp_size in
+    i*w+i' + x*w*(j*y'+j') + x*y*w*y'*(k*z'+k')
+end.
+
+Definition warp_aux (shp : shape) (id : shape) (b : Block_t shp) (f : ThreadId_t -> PhysicalId_t) :=
+  match shp,id with
+  | (x,y,z),(idx,idy,idz) => Collection ((lesser_multiple x Warp_size)/Warp_size) (fun i => Collection y (fun j => Collection z (fun k =>  warp (fun i' => f ((idx,idy,idz),(i*Warp_size+i',j,k))))))
+end.
+
+Fixpoint warps (e : execution_resource) (f : ThreadId_t -> PhysicalId_t) : execution_resource :=
+  match e with
+  | Collection n v => Collection n (fun x => warps (v x) f)
+  | grid (x,y,z) (x',y',z') g => Collection x (fun i => Collection y (fun j => Collection z (fun k => (warp_aux (x',y',z') (i,j,k) (g i j k) f))))
+  | block (x,y,z) (idx,idy,idz) b => warp_aux (x,y,z) (idx,idy,idz) b f
+  | warp w => e
+  | _ => Error
+end.
+
+Fixpoint maptranslate (f : ThreadId_t -> PhysicalId_t) (l : List execution_resource) : List execution_resource :=
+  match l with
+  | [] => []
+  | h :: tl => match h with
+               | lthread i => thread (f i)::(maptranslate f tl)
+               | _ => h::(maptranslate f tl)
+end end.
+
+Fixpoint translate (e : execution_resource) (f : ThreadId_t -> PhysicalId_t) : execution_resource :=
+  match e with
+  | Collection n v => Collection n (fun x => translate (v x) f)
+  | lthread i => thread (f i)
+  | _ => e
+end.
+
+
+(* Example test2 :
+  let f_addr := get_physical_id (1,1,1) (2,2,2) in
+  to_list (translate (for_all (for_all (for_all
+      (Block (XYZ 2 2 2)) _z) _y) _x) f_addr) =
+    [[[@ thread 0 :: @ thread 1 :: []] :: [@ thread 8 :: @ thread 9 :: []] :: []]
+ :: [[@ thread 16 :: @ thread 17 :: []] :: [@ thread 24 :: @ thread 25 :: []] :: []] :: []].
 Proof.
   simpl.
   reflexivity.
-Qed.
+Qed. *)
+
+(* Example test3 :
+  let f_addr := get_physical_id (1,1,1) (2,2,2) in
+  to_list (translate (for_all (select_range (for_all
+      (Block (XYZ 2 5 2)) _z) 2 4 _y) _x) f_addr) =
+    [[[@ thread 16 :: @ thread 17 :: []] :: [@ thread 24 :: @ thread 25 :: []] :: []]
+ :: [[@ thread 32 :: @ thread 33 :: []] :: [@ thread 40 :: @ thread 41 :: []] :: []] :: []].
+Proof.
+  simpl.
+  reflexivity.
+Qed. *)
+
+
+(* Example test4 :
+  let f_addr := get_physical_id (1,1,1) (2,2,2) in
+  to_list (for_all (warps (Block (XYZ 2 2 2)) f_addr) _x) =
+  [[[
+[@ thread 0 :: @ thread 1 :: @ thread 2 :: @ thread 3 :: @ thread 4 :: @ thread 5 :: @ thread 6 :: @ thread 7
+:: []] :: []]
+::
+[[@ thread 8 :: @ thread 9 :: @ thread 10 :: @ thread 11 :: @ thread 12 :: @ thread 13 :: @ thread 14 :: @ thread 15
+:: []] :: []]
+:: []]
+::
+[[[@ thread 16 :: @ thread 17 :: @ thread 18 :: @ thread 19 :: @ thread 20 :: @ thread 21 :: @ thread 22 :: @ thread 23
+:: []] :: []]
+::
+[[@ thread 24 :: @ thread 25 :: @ thread 26 :: @ thread 27 :: @ thread 28 :: @ thread 29 :: @ thread 30 :: @ thread 31
+:: []] :: []]
+:: []] :: []].
+Proof.
+  simpl.
+  reflexivity.
+Qed. *)
 
 
 
